theories/playground/language.v
@@ -1,0 +1,334 @@
+From iris.prelude Require Import options prelude.
+From stdpp Require Import gmap.
+
+
+Class Language := {
+  expr: Type;
+  step: expr → expr → list expr → Prop;
+  val: expr → Prop;
+  is_val:> ∀ e, Decision (val e);
+  val_no_step: ∀ e, val e → ¬ ∃ e' efs, step e e' efs;
+}.
+
+
+Notation pool := (list (expr * expr)).
+Notation delays := (list nat).
+
+(* Language Setup *)
+Notation "P '.(tgt)'" := (P.*1) (at level 5).
+Notation "P '.(src)'" := (P.*2) (at level 5).
+
+
+Section language_setup.
+
+  Context `{!Language}.
+  Implicit Types (e: expr) (T: list expr) (D: delays) (P: pool).
+
+
+  Definition no_fork e e' := step e e' [].
+  Definition no_forks e e' := rtc no_fork e e'.
+
+  Definition threads T :=
+    list_to_set (C := gset nat) (seq 0 (length T)).
+
+  Lemma threads_spec T i:
+    i ∈ threads T ↔ ∃ e, T !! i = Some e.
+  Proof.
+    rewrite elem_of_list_to_set elem_of_seq.
+    split.
+    - intros [_ Hlt]. eapply lookup_lt_is_Some_2. lia.
+    - intros ? % lookup_lt_is_Some_1. lia.
+  Qed.
+
+  Lemma threads_update T i e:
+    threads T ⊆ threads (<[i:=e]> T).
+  Proof.
+    intros j [e' Hlook]%threads_spec.
+    eapply threads_spec.
+    destruct (decide (i = j)).
+    - subst; exists e.
+      eapply list_lookup_insert, lookup_lt_Some, Hlook.
+    - rewrite list_lookup_insert_ne; last done. by exists e'.
+  Qed.
+
+  Lemma threads_weaken T T':
+    threads T ⊆ threads (T ++ T').
+  Proof.
+    intros j (e & Hlook)%threads_spec.
+    eapply threads_spec. exists e.
+    eapply lookup_app_l_Some, Hlook.
+  Qed.
+
+  Lemma threads_src_tgt P:
+    threads P.(tgt) = threads P.(src).
+  Proof.
+    by rewrite /threads !fmap_length.
+  Qed.
+
+
+
+  (* we lift the step relation to thread pools,
+    and we define the notion of a fair step.
+    A fair step decreases counters in an associated
+    delay list.
+  *)
+  Inductive pool_step : list expr → nat → list expr → Prop :=
+    take_pool_step i T_l e e' T_r T_f:
+      step e e' T_f →
+      i = length T_l →
+      pool_step (T_l ++ e :: T_r) i (T_l ++ e' :: T_r ++ T_f).
+
+  Inductive pool_steps : list expr → gset nat → list expr → Prop :=
+    | pool_no_steps T: pool_steps T ∅ T
+    | pool_do_steps T T' T'' i I J:
+      pool_step T i T' →
+      pool_steps T' I T'' →
+      J ≡ I ∪ {[i]} →
+      pool_steps T J T''.
+
+
+  Lemma pool_step_iff T i T':
+    pool_step T i T' ↔
+    (∃ e e' T_f, step e e' T_f ∧ T !! i = Some e ∧ T' = <[i := e']> T ++ T_f).
+  Proof.
+    split.
+    - destruct 1 as [i T_l e e' T_r T_f Hstep]; subst.
+      exists e, e', T_f. split; first done.
+      rewrite list_lookup_middle; last done.
+      split; first done.
+      replace (length T_l) with (length T_l + 0) by lia.
+      rewrite insert_app_r; simpl.
+      by rewrite -app_assoc.
+    - intros (e & e' & T_f & Hstep & Hlook & ->).
+      replace T with (take i T ++ e :: drop (S i) T); last by eapply take_drop_middle.
+      assert (i = length (take i T)).
+      { rewrite take_length_le; first lia. eapply lookup_lt_Some in Hlook. lia. }
+      replace i with (length (take i T) + 0) at 4 by lia.
+      rewrite insert_app_r. simpl.
+      rewrite -app_assoc; simpl.
+      econstructor; auto.
+  Qed.
+
+  Lemma pool_steps_single T i T':
+    pool_step T i T' →
+    pool_steps T {[i]} T'.
+  Proof.
+    intros Hstep; econstructor; [eauto|constructor|].
+    set_solver.
+  Qed.
+
+  Lemma pool_step_value_preservation e T i j T':
+    pool_step T j T' →
+    val e →
+    T !! i = Some e →
+    T' !! i = Some e.
+  Proof.
+    rewrite pool_step_iff.
+    destruct 1 as (e1 & e2 & T_f & Hstep & Hpre & Hpost).
+    intros Hval Hlook. destruct (decide (i = j)); subst.
+    - pose proof val_no_step. naive_solver.
+    - eapply lookup_app_l_Some.
+      rewrite list_lookup_insert_ne; done.
+  Qed.
+
+  Lemma pool_steps_value_preservation e T i J T':
+    pool_steps T J T' →
+    val e →
+    T !! i = Some e →
+    T' !! i = Some e.
+  Proof.
+    induction 1; eauto using pool_step_value_preservation.
+  Qed.
+
+  Lemma no_forks_pool_steps e e' e'' i T:
+    no_fork e e' →
+    no_forks e' e'' →
+    T !! i = Some e →
+    pool_steps T {[i]} (<[i := e'']> T).
+  Proof.
+    intros Hstep Hsteps.
+    revert e T Hstep.
+    induction Hsteps as [e'|e' e'' e''' Hstep' Hsteps IH]; intros e T Hstep Hlook.
+    - eapply pool_steps_single, pool_step_iff.
+      exists e, e', []; split; first done. split; first done.
+      by rewrite right_id.
+    - econstructor.
+      + eapply pool_step_iff. exists e, e', []; split; first done. split; first done.
+        rewrite right_id. reflexivity.
+      + rewrite -(list_insert_insert T i e''' e'). eapply IH; eauto.
+        eapply list_lookup_insert, lookup_lt_Some, Hlook.
+      + set_solver.
+  Qed.
+
+  Lemma pool_steps_set_morph T T' I J:
+    pool_steps T I T' →
+    I ≡ J →
+    pool_steps T J T'.
+  Proof.
+    by intros ? ->%leibniz_equiv.
+  Qed.
+
+  Lemma pool_steps_trans T T' T'' I I' J:
+    pool_steps T I T' →
+    pool_steps T' I' T'' →
+    I ∪ I' ≡ J →
+    pool_steps T J T''.
+  Proof.
+    induction 1 in J.
+    - intros Hsteps Heq; eapply pool_steps_set_morph; first apply Hsteps. set_solver.
+    - intros Hsteps Heq. econstructor; eauto. set_solver.
+  Qed.
+
+
+  (* an expression is active in a thread pool,
+    if it is not a value *)
+    Inductive fair_pool_step : list expr → list nat → nat → list expr → list nat → Prop :=
+      take_fair_step i T T' D D':
+      pool_step T i T' →
+      (∀ j n, j ≠ i → D !! j = Some n → ∃ n', n = S n' ∧ D' !! j = Some n') →
+      fair_pool_step T D i T' D'.
+
+    Lemma fair_pool_step_iff T D i T' D':
+      fair_pool_step T D i T' D' ↔
+        pool_step T i T' ∧ (∀ j n, j ≠ i → D !! j = Some n → ∃ n', n = S n' ∧ D' !! j = Some n').
+    Proof.
+      split; destruct 1; eauto 10 using take_fair_step.
+    Qed.
+
+    Lemma fair_pool_step_inv T D i T' D':
+      fair_pool_step T D i T' D' →
+        ∃ e e' T_f, step e e' T_f ∧
+        T !! i = Some e ∧
+        T' = <[i := e']> T ++ T_f ∧
+        (∀ j n, j ≠ i → D !! j = Some n → ∃ n', n = S n' ∧ D' !! j = Some n').
+    Proof.
+      destruct 1 as [i T T' D D' Pool Hdecr].
+      eapply pool_step_iff in Pool as (e & e' & T_f & Hstep & Hlook & Hupd).
+      eauto 10.
+    Qed.
+
+
+    Definition active_threads T :=
+      list_to_set (C := gset nat) (fmap fst (filter (λ '(i, e), ¬ val e) (imap pair T))).
+
+    Lemma active_threads_spec T i:
+      i ∈ active_threads T ↔ ∃ e, T !! i = Some e ∧ ¬ val e.
+    Proof.
+      rewrite /active_threads elem_of_list_to_set elem_of_list_fmap.
+      split.
+      - intros [[i' e] [-> Hlook]]; simpl.
+        eapply elem_of_list_filter in Hlook as [? Hlook].
+        eapply elem_of_lookup_imap in Hlook as (? & ? & Heq & ?).
+        injection Heq as ??; subst. eexists; split; eauto.
+      - intros [e [Hlook Hval]]. exists (i, e).
+        split; first done. eapply elem_of_list_filter.
+        split; first done. eapply elem_of_lookup_imap.
+        eexists _, _. split; done.
+    Qed.
+
+    Definition delays_for T D :=
+      ∀ i, i ∈ active_threads T → is_Some (D !! i).
+
+
+  CoInductive fair_div T D : Prop :=
+  | fair_div_step i T' D':
+    fair_pool_step T D i T' D' →
+    delays_for T D →
+    fair_div T' D' →
+    fair_div T D.
+
+  Inductive val_or_step : list expr → gset nat → list expr → Prop :=
+    | val_or_step_values T O:
+      (∀ i, i ∈ O → ∃ e, T !! i = Some e ∧ val e) → val_or_step T O T
+    | val_or_step_step I O T T' T'':
+        pool_steps T I T' → val_or_step T' (O ∖ I) T'' → val_or_step T O T''.
+
+  CoInductive fair_div_alt T : Prop :=
+    fair_div_alt_step T':
+    val_or_step T (threads T) T' →
+    fair_div_alt T' →
+    fair_div_alt T.
+
+  Lemma active_threads_step T i T':
+    pool_step T i T' → active_threads T ∖ {[i]} ⊆ active_threads T'.
+  Proof.
+    intros (e & e' & T_f & Hstep & Hlook & ->)%pool_step_iff.
+    intros j [Hact Hnj]%elem_of_difference.
+    eapply active_threads_spec in Hact as (e'' & Hlook' & Hnval).
+    assert (i ≠ j) by set_solver.
+    eapply active_threads_spec. exists e''; split; last done.
+    eapply lookup_app_l_Some. rewrite list_lookup_insert_ne //.
+  Qed.
+
+  Lemma threads_mono T i T':
+    pool_step T i T' → threads T ⊆ threads T'.
+  Proof.
+    intros (e & e' & T_f & Hstep & Hlook & ->)%pool_step_iff.
+    etrans; last by eapply threads_weaken.
+    eapply threads_update.
+  Qed.
+
+  Lemma threads_mono' T I T':
+    pool_steps T I T' → threads T ⊆ threads T'.
+  Proof.
+    induction 1; first done.
+    etrans; first by eapply threads_mono.
+    done.
+  Qed.
+
+  Lemma fair_div_delays T D:
+    fair_div T D → delays_for T D.
+  Proof. by destruct 1. Qed.
+
+  Lemma fair_div_active_threads_steps T D:
+    fair_div T D → ∃ T' D' O, active_threads T ⊆ O ∧ fair_div T' D' ∧ pool_steps T O T'.
+  Proof.
+    enough (∀ O T D, O ⊆ active_threads T → fair_div T D → ∃ T' D' O', O ⊆ O' ∧ fair_div T' D' ∧ pool_steps T O' T') by eauto.
+    clear T D; intros O; induction (set_wf O) as [O _ IHO]; intros T D Hsub Hfair.
+    destruct (decide (O ≡ ∅)) as [->%leibniz_equiv|[i Hi]%set_choose].
+    - exists T, D, ∅. do 2 (split; first done). constructor.
+    - assert (delays_for T D) as Hdel by by destruct Hfair.
+      assert (is_Some (D !! i)) as [d HD] by eapply Hdel, Hsub, Hi.
+      revert T D Hsub Hfair Hdel HD. induction (lt_wf d) as [d _ IHd].
+      intros T D Hsub Hfair Hdel HD. destruct Hfair as [j T' D' Hstep _ Hfair].
+      eapply fair_pool_step_iff in Hstep as [Hpool Hdecr].
+      destruct (decide (j ∈ O)).
+      + edestruct (IHO (O ∖ {[j]})) as (T'' & D'' & O' & HO' & Hfair' & Hsteps).
+        * by set_solver.
+        * etrans; last by apply active_threads_step. set_solver.
+        * apply Hfair.
+        * exists T'', D'', (O' ∪ {[j]}); split.
+         { intros k Hk; destruct (decide (k = j)); set_solver. }
+          split; first done.
+          econstructor; eauto.
+      + assert (j ≠ i) by set_solver.
+        edestruct Hdecr as (d' & Heq & HD'); eauto.
+        subst d. edestruct (IHd d') as (T'' & D'' & O' & HO' & Hfair' & Hsteps).
+        * lia.
+        * etrans; last by eapply active_threads_step. set_solver.
+        * eauto.
+        * by eapply fair_div_delays.
+        * done.
+        * exists T'', D'', (O' ∪ {[j]}); split.
+          { intros k Hk; destruct (decide (k = j)); set_solver. }
+          split; first done.
+          econstructor; eauto.
+  Qed.
+
+
+  Lemma fair_div_foo T D:
+    fair_div T D → fair_div_alt T.
+  Proof.
+    revert T D; cofix IH; intros T D Hfair.
+    eapply fair_div_active_threads_steps in Hfair as (T' & D' & O & Hsub & Hfair' & Hsteps).
+    apply (fair_div_alt_step T T'); last eauto.
+    econstructor; eauto.
+    constructor. intros i [Hi Ho]%elem_of_difference.
+    eapply threads_spec in Hi as [e Hlook].
+    destruct (decide (val e)).
+    - exists e; split; last done. by eapply pool_steps_value_preservation.
+    - exfalso. eapply Ho, Hsub, active_threads_spec. eauto 10.
+  Qed.
+
+
+End language_setup.
